trunk/color/DP/AGraph.v
@@ -1,0 +1,118 @@
+(**
+CoLoR, a Coq library on rewriting and termination.
+See the COPYRIGHTS and LICENSE files.
+
+- DucasLeo, 2007-01-22
+
+Agraph
+*)
+(** head rules graph, generalisation of ADPGraph to S @ (hd_red R)
+instead of (int_red R #) @ (dp R) *)
+
+Set Implicit Arguments.
+
+Require Export LogicUtil.
+
+Section S.
+
+Require Export ASignature.
+
+Variable Sig : Signature.
+
+Require Export ATerm.
+
+Notation term := (term Sig).
+Notation terms := (vector term).
+
+Require Export ATrs.
+
+Notation rule := (rule Sig).
+Notation rules := (list rule).
+Notation lhs := (@lhs Sig).
+Notation rhs := (@rhs Sig).
+
+Variable S : relation term.
+Variable R : rules.
+
+Variable hyp : rules_preserv_vars R.
+
+(***********************************************************************)
+
+Require Export ARename.
+
+Definition hd_red_Mod :=  S @ (hd_red R).
+
+
+
+Definition hd_rules_graph a1 a2 := In a1 R /\ In a2 R
+  /\ exists p, exists s,
+    S (app s (rhs a1)) (app s (shift p (lhs a2))).
+
+Lemma restricted_dp_graph : is_restricted hd_rules_graph R.
+
+Proof.
+unfold is_restricted, hd_rules_graph, inclusion. intros. intuition.
+Qed.
+
+(***********************************************************************)
+
+Definition hd_red_Mod_rule a t u := In a R /\
+  exists s, S t (app s (lhs a)) /\ u = app s (rhs a).
+
+Lemma chain_hd_rules_hd_red_Mod : forall a, hd_red_Mod_rule a << hd_red_Mod.
+Proof.
+unfold inclusion. intros. destruct H. do 2 destruct H0.
+exists (app x0 (lhs a)). split;auto. 
+subst y. destruct a. simpl in *. unfold hd_red. exists lhs;exists rhs;exists x0. auto.
+Qed.
+
+
+Lemma hd_red_Mod_chain_hd_rules : forall t u, hd_red_Mod t u-> exists a, hd_red_Mod_rule a t u.
+Proof.
+intros. do 2 destruct H. do 3 destruct H0.  exists (mkRule x0 x1).
+unfold hd_red_Mod_rule. simpl. intuition. exists x2. intuition.
+subst. auto.
+Qed.
+
+Lemma hd_red_Mod_rule2_hd_rules_graph : forall a1 a2 t u v,
+  hd_red_Mod_rule a1 t u -> hd_red_Mod_rule a2 u v -> hd_rules_graph a1 a2.
+
+Proof.
+intros. destruct a1 as [l0 r0]. destruct a2 as [l1 r1].
+destruct H. simpl in H1. do 2 destruct H1. subst u. rename x into s0.
+destruct H0. simpl in H2. do 2 destruct H2. subst v. rename x into s1.
+(* [maxvar l0 + 1] for shift *)
+unfold hd_rules_graph. intuition. simpl. set (p := maxvar l0 + 1). exists p.
+(* take the union of s0 (restricted to [vars l0])
+and [comp s1 (shift_inv_sub p l1)] (restricted to [vars (shift p l1)] *)
+set (s0' := restrict s0 (vars l0)).
+set (s1' := restrict (comp s1 (shift_inv_sub p l1)) (vars (shift p l1))).
+set (s := ASubstitution.union s0' s1'). exists s.
+(* compatibility *)
+assert (compat s0' s1' (vars l0) (vars (shift p l1))). unfold compat. intros.
+deduce (vars_max H3). deduce (in_vars_shift_min H4). unfold p in H6.
+absurd (x <= maxvar l0). omega. assumption.
+(* domains of substitutions *)
+assert (dom_incl s0' (vars l0)). unfold s0'. apply dom_incl_restrict.
+assert (dom_incl s1' (vars (shift p l1))). unfold s1'. apply dom_incl_restrict.
+(* inclusion in the dp_graph *)
+assert (app s r0 = app s0' r0). unfold s. eapply app_union1. apply H5. apply H3.
+apply hyp. assumption. rewrite H6.
+assert (app s0' r0 = app s0 r0). unfold s0'. symmetry.
+apply app_restrict_incl. apply hyp. assumption. rewrite H7.
+assert (app s (shift p l1) = app s1' (shift p l1)).
+unfold s. eapply app_union2. apply H4. apply H3. apply List.incl_refl.
+rewrite H8.
+assert (app s1' (shift p l1) = app s1 l1). unfold s1'.
+rewrite <- app_restrict. rewrite <- app_shift.
+refl. rewrite H9. assumption.
+Qed.
+
+
+End S.
+
+
+
+
+
+
